update Coq files for lecture

theories/type_systems/stlc/untyped.v
@@ -10,7 +10,8 @@ Lemma steps_app_r (e1 e2 e2' : expr) :
   rtc step (e1 e2) (e1 e2').
 Proof.
   induction 1 as [ e | e e' e'' Hstep Hsteps IH].
-  - reflexivity.
+  - (** [reflexivity] works not only on [=], but on reflexive relations in general. *)
+    reflexivity.
   - eapply (rtc_l _ _ (e1 e')).
     { by eapply StepAppR. }
     done.
@@ -34,7 +35,7 @@ Qed.
 
 (** We do not re-define the language to remove primitive addition -- instead, we just
   restrict our usage in this file to variables, application, and lambdas.
- *)
+*)
 
 
 Definition omega : val := lam: "x", "x" "x".
@@ -49,15 +50,27 @@ Qed.
 
 (** ** Scott encodings *)
 
-Definition zero : val := lam: "o" "s", "o".
+(** Since the Scott-encoded terms can become rather large, we also use this
+opportunity to introduce some of the automation facilities of Coq that help
+dealing with larger terms. *)
 
-Definition succ (n : val) : val := lam: "o" "s", "s" n.
+Definition zero : val := lam: "z" "s", "z".
 
 Fixpoint enc_nat (n : nat) : val :=
   match n with
   | O => zero
-  | S n => succ (enc_nat n)
+  | S n => lam: "z" "s", "s" (enc_nat n)
   end.
+
+Compute (enc_nat 1).
+
+(** [Succ] can be seen as a constructor in the language: it takes a
+representation of [n] and returns a representation of [S n]. *)
+Definition Succ : val := lam: "n" "z" "s", "s" "n".
+
+(** This computes as we would expect. *)
+Example three : step (Succ (enc_nat 2)) (enc_nat 3).
+Proof. apply StepBeta. apply is_val_of_val. Qed.
 
 (** When doing these proofs in Coq we realize that we care about whether a term
 is "closed". A term is said to be closed if all variables it mentions are bound
@@ -89,11 +102,13 @@ Proof.
   rewrite subst_closed_nil; last apply enc_nat_closed.
   reflexivity.
 Restart.
-  (** This can be automated better! All those sequences of [econstructor]
-  and [apply is_val_val] can be handled by [eauto] if we just tell it which
-  lemmas to apply. *)
-#[local] Hint Constructors step : core.
+  (** This can be automated better! We want to use the [eauto] tactic for this.
+  [eauto] can automate applying lemmas. It works with a database of known lemmas
+  and applies lemmas to the goal until the goal is solved.
+  To solve our side-conditions, we tell it about [is_val_of_val],
+  and we ask it to apply all the constructors of [step]. *)
 #[local] Hint Resolve is_val_of_val : core.
+#[local] Hint Constructors step : core.
   simpl. eapply rtc_l.
   { eauto. }
   simpl. eapply rtc_l.
@@ -115,10 +130,6 @@ Proof.
   { eauto. }
   rewrite subst_closed_nil; done.
 Qed.
-
-(** [Succ] can be seen as a constructor in the language: it takes a
-representation of [n] and returns a representation of [S n]. *)
-Definition Succ : val := lam: "n" "o" "s", "s" "n".
 
 Lemma Succ_red n : step (Succ (enc_nat n)) (enc_nat (S n)).
 Proof. econstructor; auto. Qed.
@@ -150,16 +161,22 @@ Proof.
   is pretty bad at unfolding definitions like [mul2] or [Fix]. So instead
   we directly use tactics like [econstructor] that are more expensive
   but also better at looking through definitions. [by eauto] takes
-  care of side-conditions like the [is_value] that comes up. *)
-  Ltac solve_step := repeat (simpl; econstructor; try by eauto).
-  (** When to reduce the term by one step, we apply [rtc_l] and
+  care of side-conditions like the [is_value] that comes up.
+  We [repeat] because after applying a rule such as [StepAppR],
+  we need to use another constructor to reduce a term below the application.
+
+  We do not expect you to be able to come up with tactics like this,
+  but we will provide them when they are useful and explain
+  what they do. *)
+  Ltac solve_step := repeat (econstructor; try by eauto).
+  (** To reduce the term by one step, we apply [rtc_l] and
   solve the [step] goal that this will open. *)
   Ltac one_step := eapply rtc_l; first (by solve_step); simpl.
   (** Now we can repeat that until the term is as reduced as it gets. *)
   repeat one_step. done.
 Qed.
 
-(** We prove that it satisfies the recursive unfolding. *)
+(** We prove that [fix] satisfies the recursive unfolding. *)
 Lemma Fix_step (s r : val) :
   is_closed [] s ->
   rtc step (Fix s r) (s ((Fix s))%E r).
@@ -203,4 +220,50 @@ Proof.
   do 2 one_step.
   rewrite subst_closed_nil; last done.
   by one_step.
+Qed.
+
+(** Now we can prove that [mul2] behaves the way we want. *)
+Lemma mul2_step_0 : rtc step (mul2 zero) zero.
+Proof. repeat one_step. done. Qed.
+
+Lemma mul2_step_S n : rtc step (mul2 (enc_nat (S n))) (Succ (Succ (mul2 (enc_nat n)))).
+Proof.
+  (** The [etrans] tactic works on transitive relations. It applies transitivity
+  and introduces an evar for the new term "in the middle". Here is is equivaleny
+  to (and shorter than) [eapply rtc_transitive]. *)
+  etrans.
+  { eapply Fix_step. done. }
+  (* beta-reduce [mul2_step]'s 2 arguments. *)
+  do 2 one_step.
+  (* Sadly now it becomes hard to see what we are doing, since all definitions
+  are unfolded. But we know what this is so we can [change] to a readbale goal. *)
+  change (rtc step ((enc_nat (S n)) zero (lam: "n'", Succ (Succ (mul2 "n'")))) (Succ (Succ (mul2 (enc_nat n)))))%E.
+  (* After 2 beta-reductions we have reduced away the case distinction *)
+  simpl. do 2 one_step.
+  (* This involves [subst] into the closed value [enc_nat], let's get rid of that. *)
+  rewrite (subst_closed_nil (enc_nat _)); last apply enc_nat_closed.
+  rewrite subst_closed_nil; last apply enc_nat_closed.
+  (* Now we can make the goal nice again. *)
+  change (rtc step ((lam: "n'", Succ (Succ (mul2 "n'"))) (enc_nat n)) (Succ (Succ (mul2 (enc_nat n)))))%E.
+  (* And we are just a single beta-reduction away from being done! *)
+  one_step. done.
+Qed.
+
+Lemma mul2_correct n : rtc step (mul2 (enc_nat n)) (enc_nat (2 * n)).
+Proof.
+  induction n as [|n' IH].
+  - apply mul2_step_0.
+  - etrans.
+    { apply mul2_step_S. }
+    (* Reduce the [mul2 (enc_nat n')] under the two [Succ]. *)
+    etrans.
+    { eapply steps_app_r, steps_app_r. done. }
+    (* Reduce the [Succ]. *)
+    eapply rtc_l.
+    { eapply StepAppR, Succ_red. }
+    eapply rtc_l.
+    { eapply Succ_red. }
+    (* lia helps us to shape the goal. *)
+    replace (2 * S n')%nat with (S (S (2 * n'))) by lia.
+    done.
 Qed.
